\documentclass{article}
\begin{document}
  \section{Addition}\label{sec:addition}

  \begin{forthel}
    %[prove off][check off]
    [readtex \path{dedekind.ftl.tex}]
    %[prove on][check on]
  \end{forthel}

  \begin{forthel}
    \begin{lemma}\label{add_existence}
      There exists a $\varphi : \Nat \times \Nat \to \Nat$ such
      that for all $n \in \Nat$ we have
      \[\varphi(n,0) = n\]
      and
      \[\varphi(n,\succ(m)) = \succ(\varphi(n,m))\]
      for all $m \in \Nat$.
    \end{lemma}
    \begin{proof}
      Take $A = [\Nat \to \Nat]$.
      Define $a(n) = n$ for $n \in \Nat$.
      Then $A$ is a set and $a \in A$.

      [skipfail on] % Wrong proof task %!!
      Define $f(g) = \fun n \in \Nat. \succ(g(n))$ for $g \in A$.
      [skipfail off]

      Then $f : A \to A$.
      Indeed $f(g)$ is a map from $\Nat$ to $\Nat$ for any $g \in A$.
      Consider a $\psi : \Nat \to A$ such that $\psi$ is recursively defined by
      $a$ and $f$ (by \cref{dedekind_existence}).
      Define $\varphi(n,m) = \psi(m)(n)$ for $(n,m) \in \Nat \times \Nat$.
      Then $\varphi$ is a map from $\Nat \times \Nat$ to $\Nat$.
      Indeed $\varphi(n,m) \in \Nat$ for all $n, m \in \Nat$.

      (1) For all $n \in \Nat$ we have $\varphi(n,0) = n$. \\
      Proof.
        Let $n \in \Nat$.
        Then $\varphi(n,0)
          = \psi(0)(n)
          = a(n)
          = n$.
      Qed.

      (2) For all $n, m \in \Nat$ we have $\varphi(n, \succ(m)) =
      \succ(\varphi(n,m))$. \\
      Proof.
        Let $n, m \in \Nat$.
        Then $\varphi(n, \succ(m))
          = \psi(\succ(m))(n)
          = f(\psi(m))(n)
          = \succ(\psi(m)(n))
          = \succ(\varphi(n,m))$.
      Qed.
    \end{proof}
  \end{forthel}

  \begin{forthel}
    \begin{lemma}\label{add_uniqueness}
      Let $\varphi, \varphi' : \Nat \times \Nat \to \Nat$.
      Assume that for all $n \in \Nat$ we have
      \[\varphi(n,0) = n\]
      and
      \[\varphi(n,\succ(m)) = \succ(\varphi(n,m))\]
      for all $m \in \Nat$.
      Assume that for all $n \in \Nat$ we have
      \[\varphi'(n,0) = n\]
      and
      \[\varphi'(n,\succ(m)) = \succ(\varphi'(n,m))\]
      for all $m \in \Nat$.
      Then $\varphi = \varphi'$.
    \end{lemma}
    \begin{proof}
      Define $\Phi = \{ m \in \Nat \mid \varphi(n,m) = \varphi'(n,m)$ for
      all $n \in \Nat \}$.

      (1) $0 \in \Phi$.
      Indeed $\varphi(n,0) = n = \varphi'(n,0)$ for all $n \in \Nat$.

      (2) For all $m \in \Phi$ we have $\succ(m) \in \Phi$. \\
      Proof.
        Let $m \in \Phi$.
        Then $\varphi(n,m) = \varphi'(n,m)$ for all $n \in \Nat$.
        Hence $\varphi(n, \succ(m))
          = \succ(\varphi(n,m))
          = \succ(\varphi'(n,m))
          = \varphi(n, \succ(m))$
        for all $n \in \Nat$.
      Qed.

      Thus $\Phi$ contains every natural number.
      Therefore $\varphi(n,m) = \varphi'(n,m)$ for all $n, m \in \Nat$.
    \end{proof}
  \end{forthel}
\end{document}
