\begin{forthel}
  \begin{proposition}\printlabel{ARITHMETIC_13_1097950367318016}
    Let $n$ be a natural number.
    Assume $n \geq 5$.
    Then \[ 2^{n} > n^{2}. \]
  \end{proposition}
  \begin{proof}
    Define $\Phi = \{ n' \in \Nat_{\geq 5} \mid 2^{n'} > n'^{2} \}$.

    (1) $\Phi$ contains $5$.
    Indeed $2^{5}
       = 2 \cdot (2 \cdot (2 \cdot (2 \cdot 2)))
       = (5 \cdot 5) + 7.
      > 5 \cdot 5
      = 5^{2}$.
    Indeed $((5 \cdot 5) + 7) > 5 \cdot 5$.

    (2) For all $n' \in \Phi$ we have $n' + 1 \in \Phi$. \\
    Proof.
      Let $n' \in \Phi$.
      Then $n' \geq 5$ and $2^{n'} > n'^{2}$.

      (a) $2^{n'} \cdot 2 > n'^{2} \cdot 2$.
      Indeed $2 \neq 0$.

      (b) $n'^{2} \cdot 2 = n'^{2} + n'^{2}$.

      (c) $n'^{2} + n'^{2} > n'^{2} + ((2 \cdot n') + 1)$.
      Indeed $n'^{2} > (2 \cdot n') + 1$.

      (d) $n'^{2} + ((2 \cdot n') + 1) = (n' + 1)^{2}$.

      Take $A = 2^{n' + 1}$ and $B = (n' + 1)^{2}$. %!
      Then
      \[  A                                 \]
      \[    = 2^{n' + 1}                    \]
      \[    = 2^{n'} \cdot 2                \]
      \[    > n'^{2} \cdot 2                \]  % (a)
      \[    = n'^{2} + n'^{2}               \]  % (b)
      \[    > n'^{2} + ((2 \cdot n') + 1)   \]  % (c)
      \[    = (n' + 1)^{2}                  \]  % (d)
      \[    = B.                            \]

      Thus $2^{n' + 1} = A > B = (n' + 1)^{2}$.
    Qed.

    Therefore $\Phi$ contains every element of $\Nat_{\geq 5}$.
    Consequently $2^{n} > n^{2}$.
  \end{proof}
\end{forthel}

\begin{forthel}
  \begin{proposition}\printlabel{ARITHMETIC_11_8426075493236736}
    Let $n, m, k$ be natural numbers such that $n, m \neq 0$ and $k > 1$.
    Then \[ k^{n} \mid k^{m} \iff n \leq m. \]
  \end{proposition}
  \begin{proof}
    Case $k^{n} \mid k^{m}$.
      Assume $n > m$.
      Take a nonzero natural number $l$ such that $n = m + l$.
      Then $k^{n}
        = k^{m + l}
        = k^{m} \cdot k^{l}$.
      Hence $k^{m} \mid k^{n}$.
      Thus $k^{m} = k^{n}$.
      Therefore $m = n$.
      Contradiction.
    End.

    Case $n \leq m$.
      Take a natural number $l$ such that $m = n + l$.
      Then $k^{m}
        = k^{n + l}
        = k^{n} \cdot k^{l}$.
      Hence $k^{n} \mid k^{m}$.
    End.
  \end{proof}
\end{forthel}

\begin{forthel}
  \begin{proposition}\printlabel{ARITHMETIC_11_797196163219456}
    Let $n$ be a composite natural number.
    Then $n$ has a nontrivial divisor $m$ such that $m^{2} \leq n$.
  \end{proposition}
  \begin{proof}
    Define $\Phi = \{ m \in \Nat \mid m$ is a nontrivial divisor of $n \}$.
    $A$ contains some natural number.
    Hence we can take a least natural number $m$ of $A$.
    Consider a natural number $k$ such that $m \cdot k = n$.
    Then $m \leq k$.
    Indeed if $k < m$ then $k$ is the least natural number of $A$.
    Hence $m^{2} = m \cdot m \leq m \cdot k = n$.
    Therefore $m^{2} \leq n$.
  \end{proof}
\end{forthel}

\begin{forthel}
  \begin{proposition}\printlabel{ARITHMETIC_11_2632282722533376}
    Let $k$ be a nonzero natural number.
    If $k \cdot m^{2} = n^{2}$ for some nonzero $n, m \in \Nat$ then $k$ is
    compound.
  \end{proposition}
  \begin{proof}
    Assume $k \cdot m^{2} = n^{2}$ for some nonzero $n, m \in \Nat$.
    Consider nonzero $n, m \in \Nat$ such that $k \cdot m^{2} \cdot m^{2} =
    n^{n}$.

    Case $k = 1$. Obvious.

    Case $k > 1$.
      Define $\Phi = \{ n' \in \Nat \mid$ if $n' \neq 0$ and $k \cdot m^{2} =
      n'^{2}$ then $k$ is compound $\}$.

      Let us show that for all $n' \in \Nat$ if $\Phi$ contains all
      predecessors of $n'$ then $\Phi$ contains $n'$.
        Let $n'$ be a natural number.
        Presume that $\Phi$ contains all predecessors of $n'$.
        Assume $n' \neq 0$ and $k \cdot m^{2} = n'^{2}$.

        Suppose that $k$ is prime.
        $k$ is a nontrivial divisor of $n'^{2}$.
        Hence $k$ divides $n'$.
        Take a natural number $l$ such that $k \cdot l = n'$.

        (1) Then $m^{2} = k \cdot l^{2}$.
        Indeed $k \cdot m^{2}
          = (k \cdot l)^{2}
          = k \cdot (k \cdot l^{2})$.

        (2) $m$ is an element of $\Phi$. \\
        Proof.
          We have $n'^{2} > m^{2}$.
          Indeed $k \cdot m^{2} = n'^{2}$ and $k > 1$ and $m^{2} > 0$.
          Hence $m < n'$.
          Indeed if $n' \leq m$ then $n'^{2} \leq m^{2}$.
          Thus $m \in \Phi$.
        Qed.

        (3) $l$ is nonzero.
        Indeed $l = 0 \implies
        m^{2}
          = k \cdot 0^{2}
          = k \cdot 0
          = 0$
        and $m^{2} = 0 \implies m = 0$.

        Therefore $k$ is compound (by 1, 2, 3).
        Contradiction.
      End.

      Thus $\Phi$ contains every natural number.
      Therefore $k$ is compound.
    End.
  \end{proof}
\end{forthel}

\begin{forthel}
  \begin{proposition}\printlabel{ARITHMETIC_11_8113296594960384}
    Let $n$ be a natural number.
    Assume $n \geq 2$.
    Then \[ n^{n} > n!. \]
  \end{proposition}
  \begin{proof}
    Define $\Phi = \{ n' \in \Nat_{\geq 2} \mid n'^{n'} > n'! \}$.

    (1) $\Phi$ contains $2$.

    (2) For all $n' \in \Phi$ we have $n' + 1 \in \Phi$. \\
    Proof.
      Let $n' \in \Phi$.
      Then $n' \geq 2$.

      (Claim 1) $(n' + 1)^{n'} \cdot (n' + 1) > n'^{n'} \cdot (n' + 1)$. \\
      Proof.
        We have $n' + 1 > n'$ and $n' \neq 0$.
        Thus $(n' + 1)^{n'} > n'^{n'}$.
        $n' + 1$ is nonzero.
        Hence $(n' + 1)^{n'} \cdot (n' + 1) > n'^{n'} \cdot (n' + 1)$.
      Qed.

      (Claim 2) $n'^{n'} \cdot (n' + 1) > n'! \cdot (n' + 1)$.
      Indeed $n'^{n'} > n'!$ and $n' + 1 \neq 0$.

      Hence
      \[  (n' + 1)^{n' + 1}                 \]
      \[    = (n' + 1)^{n'} \cdot (n' + 1)  \]
      \[    > n'^{n'} \cdot (n' + 1)        \]
      \[    > n'! \cdot (n' + 1)            \]
      \[    = (n' + 1)!.                    \]

      Thus $(n' + 1)^{n' + 1} > (n' + 1)!$.
    Qed.

    Therefore $\Phi$ contains every element of $\Nat_{\geq 2}$.
    Consequently $n^{n} > n!$.
  \end{proof}
\end{forthel}

\begin{forthel}
  \begin{proposition}\printlabel{ARITHMETIC_11_5413271156817920}
    Let $n$ be a natural number.
    Assume $n \geq 4$.
    Then \[ n! > 2^{n}. \]
  \end{proposition}
  \begin{proof}
    Define $\Phi = \{ n' \in \Nat_{\geq 4} \mid n'! > 2^{n'} \}$.

    (1) $\Phi$ contains $4$. \\
    Proof.
      \[  4!                                  \]
      \[    = 4 \cdot (3 \cdot 2)             \]
      \[    = 2 \cdot (2 \cdot (3 \cdot 2))   \]
      \[    = 3 \cdot (2 \cdot (2 \cdot 2))   \]
      \[    > 2 \cdot (2 \cdot (2 \cdot 2))   \]
      \[    = 2^{4}.                          \]
    Qed.

    (2) For all $n' \in \Phi$ we have $n' + 1 \in \Phi$. \\
    Proof.
      Let $n' \in \Phi$.
      Then $n' \geq 4$ and $n'! > 2^{n'}$.

      (Claim 1) $0 \neq n' + 1 > 2$.
      Indeed $n' > 1$.

      (Claim 2) $n'! \cdot (n' + 1) > 2^{n'} \cdot (n' + 1)$.

      (Claim 3) $2^{n'} \cdot (n' + 1) > 2^{n'} \cdot 2$.
      Indeed $2^{n'} \neq 0$.

      Hence
      \[  (n' + 1)!                   \]
      \[    = n'! \cdot (n' + 1)      \]
      \[    > 2^{n'} \cdot (n' + 1)   \]
      \[    > 2^{n'} \cdot 2          \]
      \[    = 2^{n' + 1}.             \]

      Thus $(n' + 1)! > 2^{n' + 1}$.
    Qed.

    Therefore $\Phi$ contains every element of $\Nat_{\geq 4}$.
    Consequently $n! > 2^{n}$.
  \end{proof}
\end{forthel}
