\documentclass[../../natural-numbers.ftl.tex]{subfiles}

\begin{document}

  \typeout{
    \begin{forthel}
      [readtex FLib/BasicNotions/src/natural-numbers/sections/01_arithmetic/02_addition.ftl.tex]

      [checkconsistency off]

      Let $k, l, m, n$ denote natural numbers.
    \end{forthel}
  }


  \section{Multiplication}

  \subsection{Axioms}

  \begin{forthel}
    \begin{signature}
      $n \cdot m$ is a natural number.
    \end{signature}

    Let the product of $n$ and $m$ stand for $n \cdot m$.

    \begin{axiom}[1st multiplication axiom]
      $n \cdot 0 = 0$.
    \end{axiom}

    \begin{axiom}[2nd multiplication axiom]
      $n \cdot (m + 1) = (n \cdot m) + n$.
    \end{axiom}
  \end{forthel}


  \subsection{Computation laws}

  \begin{forthel}
    \begin{proposition}[NN 01 03 539933]
      For all $n,m,k$ we have
      $$n \cdot (m + k) = (n \cdot m) + (n \cdot k).$$
    \end{proposition}
    \begin{proof}
      Define $P = \{ "natural number" k : n \cdot (m + k) = (n \cdot m) + (n \cdot k) "for all natural numbers" n,m \}$.

      (BASE CASE) $0$ is an element of $P$.
      Indeed for all natural numbers $n,m$ we have $n \cdot (m + 0) = n \cdot m = (n \cdot m) + 0 = (n \cdot m) + (n \cdot 0)$.

      (INDUCTION STEP) For all natural numbers $k$ we have $k \in P \implies k + 1 \in P$. \\
      Proof.
        Let $k$ be a natural number.
        Assume $k \in P$.

        For all natural numbers $n,m$ we have $n \cdot (m + (k + 1)) = (n \cdot m) + (n \cdot (k + 1))$. \\
        Proof.
          Let $n,m$ be natural numbers.

          $$n \cdot (m + (k + 1))$$
          $$= n \cdot ((m + k) + 1)$$             % 2nd addition axiom
          $$= (n \cdot (m + k)) + n$$             % 2nd multiplication axiom
          $$= ((n \cdot m) + (n \cdot k)) + n$$   % k \in P
          $$= (n \cdot m) + ((n \cdot k) + n)$$   % associativity of addition
          $$= (n \cdot m) + (n \cdot (k + 1)).$$  % 2nd multiplication axiom

          Hence the thesis.
        Qed.
      Qed.

      Therefore every natural number is contained in $P$.
    \end{proof}


    \begin{proposition}[NN 01 03 322712]
      For all $n,m,k$ we have
      $$(n + m) \cdot k = (n \cdot k) + (m \cdot k).$$
    \end{proposition}
    \begin{proof}
      Define $P = \{ "natural number" k : (n + m) \cdot k = (n \cdot k) + (m \cdot k) "for all natural numbers" n,m \}$.

      (BASE CASE) $0$ belongs to $P$.
      Indeed $(n + m) \cdot 0 = 0 = 0 + 0 = (n \cdot 0) + (m \cdot 0)$ for all natural numbers $n,m$.

      (INDUCTION STEP) For all natural numbers $k$ we have $k \in P \implies k + 1 \in P$. \\
      Proof.
        Let $k$ be a natural number.
        Assume $k \in P$.

        $(n + m) \cdot (k + 1) = (n \cdot (k + 1)) + (m \cdot (k + 1))$ for all
        natural numbers $n,m$. \\
        Proof.
          Let $n,m$ be natural numbers.
          We have $((n \cdot k) + ((m \cdot k) + n)) + m =
          (((n \cdot k) + n) + (m \cdot k)) + m$.
          Hence
          $$(n + m) \cdot (k + 1)$$
          % 2nd multiplication axiom:
          $$= ((n + m) \cdot k) + (n + m)$$
          % k \in P:
          $$= ((n \cdot k) + (m \cdot k)) + (n + m)$$
          % assoziativity of addition:
          $$= (((n \cdot k) + (m \cdot k)) + n) + m$$
          % assoziativity of addition:
          $$= ((n \cdot k) + ((m \cdot k) + n)) + m$$
          $$= (((n \cdot k) + n) + (m \cdot k)) + m$$
          % associativity of addition:
          $$= ((n \cdot k) + n) + ((m \cdot k) + m)$$
          % 2nd multiplication axiom:
          $$= (n \cdot (k + 1)) + (m \cdot (k + 1)).$$
        Qed.
      Qed.

      Thus every natural number is an element of $P$.
    \end{proof}


    \begin{proposition}[NN 01 03 866630]
      $n \cdot 1 = n$.
    \end{proposition}
    \begin{proof}
      $ n \cdot 1
      = n \cdot (0 + 1)   % commutativity of addition, 1st addition axiom
      = (n \cdot 0) + n   % 2nd multiplication axiom
      = 0 + n             % 1st multiplication axiom
      = n$.               % commutativity of addition, 1st addition axiom
    \end{proof}


    \begin{corollary}[NN 01 03 302621]
    $n \cdot 2 = n + n$.
    \end{corollary}
    \begin{proof}
      $ n \cdot 2
      = n \cdot (1 + 1)   % Definition of 2
      = (n \cdot 1) + n   % 2nd multiplication axiom
      = n + n$.           % 1 is neutral wrt. multiplication
    \end{proof}


    \begin{proposition}[NN 01 03 299637]
      For all $n,m,k$ we have
      $$n \cdot (m \cdot k) = (n \cdot m) \cdot k.$$
    \end{proposition}
    \begin{proof}
      Define $P = \{ "natural number" k : n \cdot (m \cdot k) = (n \cdot m) \cdot k "for all natural numbers" n,m \}$.

      (BASE CASE) $0$ is contained in $P$.
      Indeed for all natural numbers $n,m$ we have $n \cdot (m \cdot 0) = n \cdot 0 = 0 = (n \cdot m) \cdot 0$.

      (INDUCTION STEP) For all natural numbers $k$ we have $k \in P \implies k + 1 \in P$. \\
      Proof.
        Let $k$ be a natural number.
        Assume $k \in P$.

        For all natural numbers $n,m$ we have $n \cdot (m \cdot (k + 1)) = (n \cdot m) \cdot (k + 1)$. \\
        Proof.
          Let $n,m$ be natural numbers.
          $$n \cdot (m \cdot (k + 1))$$
          % 2nd multiplication axiom:
          $$= n \cdot ((m \cdot k) + m)$$
          % left distributivity:
          $$= (n \cdot (m \cdot k)) + (n \cdot m)$$
          % k \in P:
          $$= ((n \cdot m) \cdot k) + (n \cdot m)$$
          % 1 is neutral wrt. multiplication:
          $$= ((n \cdot m) \cdot k) + ((n \cdot m) \cdot 1)$$
          % left distributivity:
          $$= (n \cdot m) \cdot (k + 1).$$
        Qed.
      Qed.

      Hence every natural number is contained in $P$.
    \end{proof}


    \begin{proposition}[NN 01 03 850937]
      For all $n,m$ we have
      $$n \cdot m = m \cdot n.$$
    \end{proposition}
    \begin{proof}
      Define $P = \{ "natural number" m : n \cdot m = m \cdot n "for all natural"\\"numbers" n \}$.

      (BASE CASE 1) $0$ is contained in $P$. \\
      Proof.

        For all natural numbers $n$ we have $n \cdot 0 = 0 \cdot n$. \\
        Proof.
          Define $Q = \{ "natural number" n : n \cdot 0 = 0 \cdot n \}$.

          $0$ is contained in $Q$.

          For all natural numbers $n$ we have $n \in Q \implies n + 1 \in Q$. \\
          Proof.
            Let $n$ be a natural number.
            Assume $n \in Q$.
            Then
            $$
              (n + 1) \cdot 0
            = 0                 % 1st multiplication axiom
            = n \cdot 0         % 1st multiplication axiom
            = 0 \cdot n         % n \in Q
            = (0 \cdot n) + 0   % 1st addition axiom
            = 0 \cdot (n + 1).  % 2nd multiplication axiom
            $$
          Qed.
        Qed.
      Qed.

      (BASE CASE 2) $1$ belongs to $P$. \\
      Proof.
        Let us show that for all natural numbers $n$ we have $n \cdot 1 = 1 \cdot n$.
          Define $Q = \{ "natural number" n : n \cdot 1 = 1 \cdot n \}$.

          $0$ is contained in $Q$.

          For all natural numbers $n$ we have $n \in Q \implies n + 1 \in Q$. \\
          Proof.
            Let $n$ be a natural number.
            Assume $n \in Q$.
            Then
            $$  (n + 1) \cdot 1$$
            $$= (n \cdot 1) + 1$$   % right-distributivity,
            $$= (1 \cdot n) + 1$$   % 1 \in Q
            $$= 1 \cdot (n + 1).$$  % left-distributivity
          Qed.

          Thus every natural number is contained in $Q$.
          Hence the thesis.
        End.
      Qed.

      (INDUCTION STEP) For all natural numbers $m$ we have $m \in P \implies m + 1 \in P$. \\
      Proof.
        Let $m$ be a natural number.
        Assume $m \in P$.

        For all natural numbers $n$ we have $n \cdot (m + 1) = (m + 1) \cdot n$. \\
        Proof.
          Let $n$ be a natural number.
          Then
          $$n \cdot (m + 1)$$
          % left distributivity:
          $$= (n \cdot m) + (n \cdot 1)$$
          % 1,m \im P:
          $$= (m \cdot n) + (1 \cdot n)$$
          % commutativity of addition:
          $$= (1 \cdot n) + (m \cdot n)$$
          % right distributivity:
          $$= (1 + m) \cdot n$$
          % commutativity of addition:
          $$= (m + 1) \cdot n.$$
        Qed.
      Qed.

      Hence every natural number is contained in $P$.
    \end{proof}


    \begin{proposition}[NN 01 03 692941]
      For all $n,m$ we have
      $$n \cdot m = 0 \implies (n = 0 "or" m = 0).$$
    \end{proposition}
    \begin{proof}
      Let $n,m$ be natural numbers.
      Assume $n \cdot m = 0$.

      If $n$ and $m$ are not equal to $0$ then we have a contradiction. \\
      Proof.
        Assume $n,m \neq 0$.
        Take natural numbers $n',m'$ such that $n = (n' + 1)$ and $m = (m' + 1)$.
        Then
        $$0$$
        $$= n \cdot m$$
        $$= (n' + 1) \cdot (m' + 1)$$
        $$= ((n' + 1) \cdot m') + (n' + 1)$$
        $$= (((n' + 1) \cdot m') + n') + 1.$$
        Hence $0 = k + 1$ for some natural number $k$.
        Contradiction.
      Qed.

      Thus $n = 0$ or $m = 0$.
    \end{proof}


    \begin{proposition}[NN 01 03 799692]
      Assume $k \neq 0$.
      Then for all $n,m$ we have
      $$n \cdot k = m \cdot k \implies n = m.$$
    \end{proposition}
    \begin{proof}
      Define $P = \{ "natural number" n : "for all natural numbers" m "if" n \cdot k = m \cdot k "and" k \neq 0 "then" n = m \}$.

      (BASE CASE) $0$ is contained in $P$. \\
      Proof.
        Let us show that for all natural numbers $m$ if $0 \cdot k = m \cdot k$ and $k \neq 0$ then $0 = m$.
          Let $m,k$ be natural numbers.
          Assume that $0 \cdot k = m \cdot k$ and $k \neq 0$.
          Then $m \cdot k = 0$.
          Hence $m = 0$ or $k = 0$.
          Thus $m = 0$.
        End.
      Qed.

      (INDUCTION STEP) For all natural numbers $n$ we have $n \in P \implies n + 1 \in P$. \\
      Proof.
        Let $n$ be a natural number.
        Assume $n \in P$.

        For all natural numbers $m$ if $(n + 1) \cdot k = m \cdot k$ and $k \neq 0$ then $n + 1 = m$. \\
        Proof.
          Let $m$ be natural numbers.
          Assume $(n + 1) \cdot k = m \cdot k$ and $k \neq 0$.

          Case $m = 0$.
            Then $(n + 1) \cdot k = 0$.
            Hence $n + 1 = 0$.
            Contradiction.
          End.

          Case $m \neq 0$.
            Take a natural number $m'$ such that $m = m' + 1$.
            Then $(n + 1) \cdot k = (m' + 1) \cdot k$.
            Hence $(n \cdot k) + k = (m' \cdot k) + k$.
            Thus $n \cdot k = m' \cdot k$ (by NN 01 02 882987).
            Then we have $n = m'$.
            Therefore $n + 1 = m' + 1 = m$.
          End.
        Qed.
      Qed.

      Thus every natural number is contained in $P$.
    \end{proof}


    \begin{corollary}[NN 01 03 169506]
      Assume $k \neq 0$.
      Then for all $n,m$ we have
      $$k \cdot n = k \cdot m \implies n = m.$$
    \end{corollary}
    \begin{proof}
      Let $n,m$ be natural numbers.
      Assume $k \cdot n = k \cdot m$.
      We have $k \cdot n = n \cdot k$ and $k \cdot m = m \cdot k$.
      Hence $n \cdot k = m \cdot k$.
      Thus $n = m$.
    \end{proof}
  \end{forthel}
\end{document}
